new/proof/go_etcd_io/raft/v3_proof/base.v
@@ -1,0 +1,101 @@
+Require Export New.code.go_etcd_io.raft.v3.
+Require Export New.generatedproof.go_etcd_io.raft.v3.
+Require Export New.proof.proof_prelude.
+Require Export New.proof.context New.proof.sync.
+
+
+Section init.
+Context `{hG: heapGS Σ, !ffi_semantics _ _}.
+Context `{!goGlobalsGS Σ}.
+Context  `{!quorum.GlobalAddrs}.
+Context  `{!tracker.GlobalAddrs}.
+Context  `{!raft.GlobalAddrs}.
+
+#[global]
+Program Instance is_pkg_init_raftpb : IsPkgInit raftpb :=
+  ltac2:(build_pkg_init ()).
+#[global] Opaque is_pkg_init_raftpb.
+
+#[global]
+Program Instance is_pkg_init_strconv : IsPkgInit strconv :=
+  ltac2:(build_pkg_init ()).
+#[global] Opaque is_pkg_init_strconv.
+
+#[global]
+Program Instance is_pkg_init_slices : IsPkgInit slices :=
+  ltac2:(build_pkg_init ()).
+#[global] Opaque is_pkg_init_slices.
+
+#[global]
+Program Instance is_pkg_init_strings : IsPkgInit strings :=
+  ltac2:(build_pkg_init ()).
+#[global] Opaque is_pkg_init_strings.
+
+#[global]
+Program Instance is_pkg_init_math : IsPkgInit math :=
+  ltac2:(build_pkg_init ()).
+#[global] Opaque is_pkg_init_math.
+
+#[global]
+Program Instance is_pkg_init_fmt : IsPkgInit fmt :=
+  ltac2:(build_pkg_init ()).
+#[global] Opaque is_pkg_init_fmt.
+
+#[global]
+Program Instance is_pkg_init_quorum : IsPkgInit quorum :=
+  ltac2:(build_pkg_init ()).
+#[global] Opaque is_pkg_init_quorum.
+
+#[global]
+Program Instance is_pkg_init_tracker : IsPkgInit tracker :=
+  ltac2:(build_pkg_init ()).
+#[global] Opaque is_pkg_init_tracker.
+
+#[global]
+Program Instance is_pkg_init_confchange : IsPkgInit confchange :=
+  ltac2:(build_pkg_init ()).
+#[global] Opaque is_pkg_init_confchange.
+
+#[global]
+Program Instance is_pkg_init_big : IsPkgInit big :=
+  ltac2:(build_pkg_init ()).
+#[global] Opaque is_pkg_init_big.
+
+#[global]
+Program Instance is_pkg_init_rand : IsPkgInit rand :=
+  ltac2:(build_pkg_init ()).
+#[global] Opaque is_pkg_init_rand.
+
+#[global]
+Program Instance is_pkg_init_bytes : IsPkgInit bytes :=
+  ltac2:(build_pkg_init ()).
+#[global] Opaque is_pkg_init_bytes.
+
+#[global]
+Program Instance is_pkg_init_os : IsPkgInit os :=
+  ltac2:(build_pkg_init ()).
+#[global] Opaque is_pkg_init_os.
+
+#[global]
+Program Instance is_pkg_init_log : IsPkgInit log :=
+  ltac2:(build_pkg_init ()).
+#[global] Opaque is_pkg_init_log.
+
+#[global]
+Program Instance is_pkg_init_io : IsPkgInit io :=
+  ltac2:(build_pkg_init ()).
+#[global] Opaque is_pkg_init_io.
+
+#[global]
+Program Instance is_pkg_init_errors : IsPkgInit errors :=
+  ltac2:(build_pkg_init ()).
+#[global] Opaque is_pkg_init_errors.
+
+Definition foo := ltac2:(build_pkg_init ()).
+
+#[global]
+Program Instance is_pkg_init_raft : IsPkgInit raft :=
+  ltac2:(build_pkg_init ()).
+#[global] Opaque is_pkg_init_raft.
+
+End init.
