new/proof/go_etcd_io/raft/v3_proof/protocol.v
@@ -1,0 +1,122 @@
+Require Import New.proof.go_etcd_io.raft.v3_proof.base.
+Require Import New.proof.chan.
+Local Transparent is_pkg_init_raft.
+
+Module node.
+Axiom t : Type.
+End node.
+
+Module message.
+Axiom t : Type.
+End message.
+
+Module entry.
+Definition t : Type := list w8.
+End entry.
+
+Module astate.
+Record t :=
+  {
+    log : list entry.t;
+  }.
+End astate.
+
+Section raft.
+Context `{hG: heapGS Σ, !ffi_semantics _ _}.
+Context `{!goGlobalsGS Σ}.
+Context `{!quorum.GlobalAddrs}.
+Context `{!tracker.GlobalAddrs}.
+Context `{!raft.GlobalAddrs}.
+Context `{!closeable_chanG Σ}.
+Context `{!contextG Σ}.
+
+Axiom is_chan_inv : ∀ (c : chan.t) {V} `{!IntoVal V} (P : V → iProp Σ), iProp Σ.
+Instance is_chan_inv_pers c V `{!IntoVal V} (P : V → _) : Persistent (is_chan_inv c P).
+Proof. Admitted.
+
+Local Definition is_Node_inner (n : raft.node.t) : iProp Σ :=
+  "#Hpropc" ∷ is_chan_inv n.(raft.node.propc') (λ (_ : raft.msgWithResult.t), True)%I ∗
+  "#Hadvancec" ∷ is_chan_inv n.(raft.node.advancec') (λ (_ : unit), True)%I ∗
+  "#Hdone" ∷ own_closeable_chan n.(raft.node.done') True closeable.Unknown.
+
+Definition is_Node (n : loc) : iProp Σ :=
+  ∃ nd,
+  "n_ptr" ∷ n ↦□ nd ∗
+  "Hinner" ∷ is_Node_inner nd.
+
+Lemma wp_node__Ready (n : loc) :
+  {{{ is_pkg_init raft ∗ is_Node n }}}
+    n@raft@"node'ptr"@"Ready" #()
+  {{{ (ready : chan.t), RET #ready; True }}}.
+Proof.
+  wp_start. wp_auto. (* need repr predicate for node *)
+Admitted.
+
+Lemma wp_node__Advance (n : loc) :
+  {{{ is_pkg_init raft ∗ is_Node n }}}
+    n@raft@"node'ptr"@"Advance" #()
+  {{{ RET #(); True }}}.
+Proof.
+  wp_start. wp_auto.
+  iNamed "Hpre".
+  wp_auto.
+  (* FIXME: want unit, but ending up with raft.TracingEvent.t *)
+  wp_apply wp_chan_select_blocking.
+  rewrite big_andL_cons big_andL_singleton.
+  iSplit.
+  - (* able to send on advancec *)
+    repeat iExists _. instantiate (1:=(tt : unit)). iSplitR.
+    { iPureIntro. admit. }
+    Unshelve. 2: tc_solve.
+    admit. (* just prove the send atomic update then trivial postcondition *)
+  - repeat iExists _. iNamed "Hinner". Search own_closeable_chan.
+    iApply (closeable_chan_receive with "Hdone").
+    iIntros "[_ _]". wp_auto. iApply "HΦ". done.
+Admitted.
+
+Lemma wp_node__Propose n (ctx : context.Context.t) ctx_desc (data_sl : slice.t) (data : list w8) :
+  {{{ is_pkg_init raft ∗
+      "#Hctx" ∷ is_Context ctx ctx_desc ∗
+      "#Hnode" ∷ is_Node n ∗
+      "data_sl" ∷ data_sl ↦* data }}}
+    n@raft@"node'ptr"@"Propose" #ctx #data_sl
+  {{{ (err : error.t), RET #err; if decide (err = interface.nil) then False else True }}}.
+Proof.
+  (* Inlining proofs of [stepWait] and [stepWithWaitOption (wait:=true)] here. *)
+  wp_start. iNamed "Hpre". wp_auto.
+  wp_apply wp_slice_literal. iIntros "%entries_sl entries_sl".
+  wp_auto. wp_bind. wp_method_call. wp_call.
+  iClear "n ctx". clear n_ptr ctx_ptr.
+  wp_auto. wp_bind. wp_method_call. wp_call.
+  iClear "n m ctx". clear n_ptr m_ptr ctx_ptr.
+  wp_auto. iNamed "Hnode". wp_auto. wp_apply (wp_chan_make (V:=error.t)).
+  iIntros "%result %result_init Hch". wp_auto.
+  iNamed "Hctx". wp_apply "HDone".
+  wp_apply wp_chan_select_blocking.
+  rewrite !big_andL_cons big_andL_nil. rewrite right_id.
+  iSplit.
+  2:{
+    iSplit.
+    - (* case: got something from ctx.Done() channel *)
+      repeat iExists _.
+      iApply (closeable_chan_receive with "HDone_ch").
+      iIntros "[_ #HDone_closed]". wp_auto. wp_apply ("HErr" with "HDone_closed").
+      iIntros (err) "%Herr". wp_auto.
+      iApply "HΦ". rewrite decide_False //.
+    - (* case: raft is done *)
+      repeat iExists _. iNamed "Hinner".
+      iApply (closeable_chan_receive with "Hdone").
+      iIntros "[_ #HDone_closed]". wp_auto. wp_globals_get.
+      (* FIXME: global variable holding an error *)
+      admit.
+  }
+  repeat iExists _.
+  iSplitR; first done.
+Qed.
+
+End raft.
+
+Section proof.
+Context `{!heapGS Σ}.
+
+End proof.
