new/should_build.v
@@ -2,7 +2,7 @@ From New.generatedproof.github_com.goose_lang.goose.testdata.examples
   Require unittest semantics unittest.externalglobals.
 (* required just to make sure this demo works *)
 From New.golang.theory Require static_mem.
-From New.proof Require go_etcd_io.etcd.raft.v3.
+From New.proof Require go_etcd_io.raft.v3.
 From New.proof.github_com.mit_pdos.gokv Require partialapp asyncfile lockservice globals_test.
 From New.proof.github_com.goose_lang.goose.testdata.examples
   Require unittest unittest.generics.
